\documentclass{article}
\usepackage[utf8]{inputenc}
\usepackage{amsmath}
\title{Proof}
\author{Automatic WZ-method prover}
\date{2019-11-19}
\begin{document}
\maketitle
We want to prove that
\begin{equation}\label{Eq: 1}
\sum_{k=n}^{\infty} \frac{1}{\binom{k}{n}} = \frac{n}{n-1}
\end{equation}
holds.By dividing equation \ref{Eq: 1} by the right hand side we get
\begin{equation}
F(n,k)=(((1)/(B[k,n])))/(((n)/(n-1)))
\end{equation}
By using
\begin{equation}
G(n,k)=(-4n^4+(8(k-1)+4)n^3-(5(k-1)^2+8(k-1)+1)n^2+((k-1)^3+5(k-1)^2+2(k-1))n-((k-1)^3+(k-1)^2))((((1)/(B[(k-1),n])))/(((n)/(n-1))))/(2n^4-(3(k-1)+3)n^3+((k-1)^2+5(k-1)+1)n^2-(2(k-1)^2+2(k-1))n+(k-1)^2),
\end{equation}
the automatic solver has  shown that
\begin{equation}
F(n+1,k)-F(n,k)=G(n,k+1)-G(n,k).
\end{equation}
The user now has to verify that
\begin{equation}
\lim_{k\to\pm\infty}G(n,k)=0\forall n.
\end{equation}
\end{document}